Reorder events in HeapLang to match paper (+ some neat refactoring).

src/heaplang/adequacy.v
@@ -5,27 +5,35 @@ From iris.itree Require Import wpi ub itree choice state later handler void.
 From iris.itree.threadpool Require Import ctrace handler interleaving.
 From iris.itree.heaplang Require Import lang.
 
+(** An execution outcome of a HeapLang program. *)
+Definition Outcome R : Type :=
+  (state * (R + last_thread_killed + ub_crash)) + later_exhausted.
+(** An execution of a HeapLang program. *)
+Definition Execution R : Type :=
+  itree voidE (Outcome R).
+
 Definition heaplang_irel {R} (σ : state) (n : option nat) (t : itree heaplangE R)
-  (te : itree voidE ((state * (R + last_thread_killed)) + later_exhausted + ub_crash)) : Prop :=
-  ∃ t1 t2 t3,
+  (te : Execution R) : Prop :=
+  ∃ t1 t2 t3 t4,
     threadpool_irel t t1 ∧
-    demonic_irel t1 t2 ∧
+    ub_irel t1 t2 ∧
     state_irel σ t2 t3 ∧
-    te = ub_ifn (insert_voidE (later_ifn n t3)).
+    demonic_irel t3 t4 ∧
+    later_irel n (insert_voidE t4) te.
 
 Definition heaplang_eval (e : expr) (σ : state) (n : option nat)
   (* TODO: Can remove the itree here? How would we represent diverging
   programs when not using later? *)
-  (exec: itree voidE ((state * (val + last_thread_killed)) + later_exhausted + ub_crash)) : Prop :=
+  (exec: Execution val) : Prop :=
   heaplang_irel σ n (compile_expr_yield e) exec.
 
 Definition relationally_adequate (n : option nat) (e : expr) (σ : state) (φ : val → Prop) : Prop :=
   ∀ te, heaplang_eval e σ n te → ∃ x, te ≈ Ret x ∧
     match x with
-    | inr UbCrash => False
-    | inl (inr LaterExhausted) => is_Some n
-    | inl (inl (σ, inl v)) => φ v
-    | inl (inl (σ, inr _)) => True
+    | inr LaterExhausted => is_Some n
+    | inl (_, inr UbCrash) => False
+    | inl (_, inl (inl v)) => φ v
+    | inl (_, inl (inr _)) => True
     end.
 
 (** Intuitively, [e] is totally adequate with respect to heap [σ] and
@@ -65,22 +73,25 @@ Section adequacy.
     WPi t @ heaplangH m; ⊤ {{ Φ }} -∗
     |={⊤, ∅}=> ∃ x, ⌜te ≈ Ret x⌝ ∗
       match x with
-      | inr UbCrash => False
-      | inl (inr LaterExhausted) => ⌜is_Some n⌝
-      | inl (inl σr) => |={∅, ⊤}=> let (σ, r) := σr in state_interp σ ∗
-          match r with | inl v => Φ v | inr _ => True end
+      | inr LaterExhausted => ⌜is_Some n⌝
+      | inl (_, inr UbCrash) => |={∅, ⊤}=> False
+      | inl (σ, inl (inl v)) => |={∅, ⊤}=> state_interp σ ∗ Φ v
+      | inl (σ, inl (inr LastThreadKilled)) => |={∅, ⊤}=> state_interp σ
       end.
   Proof.
-    iIntros ((?&?&?&?&?&?&Hte)) "Hlc Hs Hwp".
+    iIntros ((?&?&?&?&?&->&?&?&->)) "Hlc Hs Hwp".
     iDestruct (threadpool_adequacy with "Hwp") as "Hwp"; [done|].
-    iDestruct (demonic_adequacy with "Hwp") as "Hwp"; [done|].
-    iDestruct (state_adequacy with "Hs Hwp") as "Hwp"; [done|].
-    rewrite -wpi_clear_mask. iMod "Hwp".
-    iDestruct (later_adequacy_empty with "Hlc Hwp") as "Hwp".
-    iDestruct (wpi_insert_voidE with "Hwp") as "Hwp".
     iDestruct (ub_adequacy with "Hwp") as "Hwp".
+    iDestruct (state_adequacy with "Hs Hwp") as "Hwp"; [done|].
+    iDestruct (demonic_adequacy with "Hwp") as "Hwp"; [done|].
+    rewrite -wpi_clear_mask. iMod "Hwp".
+    iDestruct (wpi_insert_voidE with "Hwp") as "Hwp".
+    iDestruct (later_adequacy_empty with "Hlc Hwp") as "Hwp".
     iApply void_adequacy_empty.
-    by rewrite Hte.
+    iApply wpi_wand; last done.
+    iIntros (?) "HΦ". repeat case_match; eauto.
+    - by iMod "HΦ" as "[$ _]".
+    - by iMod "HΦ" as "[_ $]".
   Qed.
 
   Lemma wp_adequacy_eval e σ te (Φ : val → iProp Σ) n m :
@@ -91,10 +102,10 @@ Section adequacy.
     WP e @ m; ⊤ {{ Φ }} -∗
     |={⊤, ∅}=> ∃ x, ⌜te ≈ Ret x⌝ ∗
       match x with
-      | inr UbCrash => False
-      | inl (inr LaterExhausted) => ⌜is_Some n⌝
-      | inl (inl σr) => |={∅, ⊤}=> let (σ, r) := σr in state_interp σ ∗
-          match r with | inl v => Φ v | inr _ => True end
+      | inr LaterExhausted => ⌜is_Some n⌝
+      | inl (_, inr UbCrash) => |={∅, ⊤}=> False
+      | inl (σ, inl (inl v)) => |={∅, ⊤}=> state_interp σ ∗ Φ v
+      | inl (σ, inl (inr LastThreadKilled)) => |={∅, ⊤}=> state_interp σ
       end.
   Proof.
     iIntros (?) "Hlc Hs Hinv Hwp".
@@ -124,6 +135,7 @@ Section soundness.
     iMod "Had" as "[_ %Had]".
     iApply fupd_mask_intro; first done. iIntros "_ !>". iPureIntro.
     simplify_eq. split; first done. by repeat case_match.
+    iMod "Had" as "[]".
   Qed.
 
   Lemma wp_total_soundness e σ φ :
@@ -141,6 +153,7 @@ Section soundness.
     iExists x. repeat case_match; eauto.
     - iMod "Had" as "[_ %Hφ]".
       iApply fupd_mask_intro; first done. by iIntros "_".
+    - by iMod "Had" as "%Had".
     - iDestruct "Had" as "%Had". destruct Had as [? [=]].
   Qed.
 End soundness.
@@ -160,31 +173,28 @@ Section trace.
   Context {R : Type}.
 
   (** Extract a trace for the interpreted ITree. *)
-  Definition interp_tr_heaplang σ n (tr : ctrace sequential_heaplangE R) : option (trace voidE ((state * (R + last_thread_killed)) + later_exhausted + ub_crash)) :=
-    (λ tr', interp_tr_ub (insert_voidE_tr (interp_tr_later n tr'))) <$> (interp_tr_state σ (interp_tr (sequencify tr))).
+  Definition interp_tr_heaplang σ n (tr : ctrace sequential_heaplangE R) : option (trace voidE (Outcome R)) :=
+    interp_tr_later n <$> (insert_voidE_tr <$> (interp_tr <$> (interp_tr_state σ (interp_tr_ub (sequencify tr))))).
 
   (** Construct a relational interpretation from a trace. *)
   Lemma heaplang_trace (tr : ctrace sequential_heaplangE R) (t : itree heaplangE R) tr' σ n :
     interp_tr_heaplang σ n tr = Some tr' →
     is_ctrace tr 0 [t] →
-    ∃ (te : itree voidE ((state * (R + last_thread_killed)) + later_exhausted + ub_crash)),
+    ∃ (te : Execution R),
       heaplang_irel σ n t te ∧ is_trace tr' te.
   Proof.
     intros Heq Htr.
     rewrite /interp_tr_heaplang in Heq.
-    destruct (interp_tr_state σ (interp_tr (sequencify tr))) as [tr''|] eqn:Heq'; try discriminate.
+    destruct (interp_tr_state σ (interp_tr_ub (sequencify tr))) as [tr''|] eqn:Heq'; try discriminate.
     simpl in Heq. injection Heq as <-.
     apply threadpool_trace in Htr as (t1&Hint&Htr).
-    eapply demonic_trace in Htr as (t2&Hinst&Htr).
-    apply state_trace with (s := σ) (tr' := tr'') in Htr as (t3&Heval&Htr); last done.
-    apply later_trace with (n := n) in Htr.
+    apply ub_trace in Htr as (t2&Hub&Htr).
+    apply state_trace with (s := σ) (tr' := tr'') in Htr as H; last done.
+    clear Htr. destruct H as (t3&Hst&Htr).
+    eapply demonic_trace in Htr as (t4&Hinst&Htr).
     apply insert_voidE_trace in Htr.
-    apply ub_trace in Htr.
-    exists (ub_ifn (insert_voidE (later_ifn n t3))). split; last done.
-    exists t1, t2, t3.
-    split; first done.
-    split; first done.
-    split; first done.
-    done.
+    apply later_trace with (n := n) in Htr as (t5&Hlat&Htr).
+    exists t5. split; last done.
+    by exists t1, t2, t3, t4.
   Qed.
 End trace.
